2024-04-26 Fiddler
==================
If player A's total is $a$, then player B spins once if $b > a$, where $b$
is player B's first spin, and spins twice if $b < a$.  The edge cases where
$b = a$ or other spins or sums of spins are equal are irrelevant for these
calculations.  The probability that B wins on the first spin is $1-a$.
Otherwise, B must spin at least $a-b$ and no more than $1-b$ to win
on the second spin, which has probability $1-a$.  So, given $a < 1$, the
probability that B wins is $1-a^2$.

If player A's first spin is $a_1$, the probability of losing without a
second spin is $1-a_1^2$.  When spinning twice, the probability of
immediately losing is $a_1$, otherwise, the second spin is $a_2 < 1-a_1$
and the probability of losing is then $1-(a_1+a_2)^2$.  So, given $a_1$,
the probability of losing after spinning twice is

$$ a_1 + \int_0^{1-a_1} da_2 (1 - (a_1+a_2)^2) = a_1 + (1-a_1)^2(2+a_1)/3 $$

So player A should spin twice if the first spin is less than $x$, where
$1 - x^2 = x + (1-x)^2(2+x)/3$, or $x \approx 0.53209.  There
are three real roots to $x^3 + 3x^2 - 1 = 0$, and one
of the roots is between zero and one, which is the relevant root.

So the probability of losing is

$$ \int_0^x da (a + (1-a)^2(2+a)/3) + \int_x^1 da (1-a^2)
  = 2/3 - x/3 + x^3/3 + x^4/12 $$

which is minimized when $x = 2\cos(2\pi/9) - 1 \approx 0.53209$ at
approximately 54.62%, so the probability of winning is approximately 45.38%.

Extra credit
------------
If player B's first spin is less than the greater of $a$ and $x$, where
$a$ is player A's result and $x \approx 0.53209$, player B will make a
second spin.

If $a < x$, the probability that player B does not make a second spin is $1-x$.
What player C does is irrelevant, since player A loses.

The probability that player B's result is less than $a$ after two spins
is $\int_0^a db (a-b) = a^2-a^2/2 = a^2/2$, in which case the probability
that player C wins is $1-a^2$.

The probability that player B's result is greater than 1 is
$\int_0^x db b = x^2/2$, in which case the probability that player C wins
is $1-a^2$.

The probability that player B's result is between $a$ and 1 after two spins is
$\int_0^a db (1-a) + \int_a^x db (1-b) = -a^2/2 + x - x^2/2$.

The probability that player A loses when $a < x$ is then

$$ 1-x + (a^2/2+x^2/2)(1-a^2) - a^2/2 + x - x^2/2 = 1 - x^2a^2/2 - a^4/2 $$

If $a > x$, the probability that player B does not make a second spin is $1-a$.

The probability that player B's result is less than $a$ after two spins is
$a^2/2$.

The probability that player B's result is greater than 1 is
$\int_0^a db b = a^2/2$.

The probability that player B's result is between $a$ and 1 after two spins is
$\int_0^a db (1-a) = a(1-a)$.

The probability that player A loses when $a > x$ is then

$$ 1-a + a^2(1-a^2) + a-a^2 = 1 - a^4 $$

I'll conjecture that player A spins twice if the first spin $a < y$ for
some $y$ where $x < y < 1$.  The probability that player A loses is then

$$ \int_0^x da \left(a
                + \int_0^{x-a} da_2 (1 - x^2(a+a_2)^2/2 - (a+a_2)^4/2)
                + \int_{x-a}^{1-a} da_2 (1 - (a+a_2)^4)
               \right)
   \int_x^y da \left(a
                + \int_{0}{1-a} da_2 (1 - (a+a_2)^4)
               \right)
   \int_y^1 da (1 - a^4)
$$

Evaluating with Wolfram Alpha gives

$$ 1/120 (-5 x^6 + 4 y^6 + 24 y^5 - 24 y + 96) $$

which has a minimum of approximately 69.48% at $y \approx 0.64865$,
so the probability of winning is 30.52%.

Further thoughts
----------------
One possible variation is that each player can spin any number of times, and
the number is the sum of all the spins.

If player A's result is $a$, and player B's current sum is $b < a$, player B's
probability of winning is

$$ P(a,b) = 1-a + \int_0^{a-b} ds P(a,b+s) = 1-a + \int_b^a dt P(a,t) $$

Taking the derivative with respect to $b$,

$$ \frac{dP}{db} = -P $$

so $P = Ce^{-b}$ and

$$ Ce^{-b} = 1-a + \int_b^a dx Ce^{-b} = 1-a - Ce^{-a} + Ce^{-b} $$

so $C = (1-a)e^a$, and $P = (1-a)e^{a-b}$.

Then, the total probability that player B wins is

$$ 1-a + \int_0^a db(1-a)e^{a-b} = (1-a)e^a $$

If while player A's total, $a$, is less than $x$, player A continues to spin,
the probability that player A loses is

$$ L(a,x) = a + \int_a^x ds L(a,s) + \int_x^1 ds (1-s)e^s $$

$$ L(a,x) = a + e + (x-2)e^x + \int_a^x ds L(a,s) $$

Taking the derivative with respect to $a$,

$$ \frac{dL}{da} = 1 - L $$

So $L = 1 + Ce^{-a}$ and

$$ 1 + Ce^{-a} = a + e + (x-2)e^x + x - a - Ce^{-x} + Ce^{-a} $$

so $C = e^x (e^x (x - 2) + x + e - 1)$

The total probability that player A loses is

$$ \int_0^x ds (1 + Ce^{-s}) + \int_x^1 ds (1-s)e^s
  = C (1 - e^{-x}) - 2 e^x + (e^x + 1) x + e $$

or

$$ e^{2 x} (x - 2) + e^x (x + e - 1) + 1 $$

which is minimized at approximately 57.50% when $x \approx 0.5705565$,
so the probability that player A wins is approximately 42.50%.
