2021-07-30 Riddler Classic
==========================
Link n is at an angle ğœƒ<sub>n</sub> = nğœƒ, where n=0,1,2...

That means link n+1 starts at
  x<sub>n+1</sub> = x<sub>n</sub> + f<sup>n</sup>cos(nğœƒ)
  y<sub>n+1</sub> = y<sub>n</sub> + f<sup>n</sup>sin(nğœƒ)

The curve is mapped out by x<sub>âˆ</sub>(f,ğœƒ), y<sub>âˆ</sub>(f,ğœƒ), for
ğœƒ varying from 0 to 2ğœ‹ and parameterized by f.

Consider select values of ğœƒ to try getting a sense of the curve.

At ğœƒ=0, x=1/(1-f), y=0.

At ğœƒ=ğœ‹, x=1/(1+f), y=0.

At ğœƒ=ğœ‹/2, x=1/(1+f<sup>2</sup>), y=f/(1+f<sup>2</sup>).

At ğœƒ=3ğœ‹/2, x=1/(1+f<sup>2</sup>), y=-f/(1+f<sup>2</sup>).

After plotting the 300th link for a few values values of f, it looks a lot
like a circle.

Based on the positions at ğœƒ=0 and ğœƒ=ğœ‹, if it is a circle,
the center of the circle would be at (1/(1-f<sup>2</sup>),0)
and the radius would be f/(1-f<sup>2</sup>).

Proof
-----
Consider the distance from the center of the hypothetical circle

  dx = \sum_{n=0}^\infty f^n cos(nğœƒ) - 1/(1-f^2)
  dy = \sum_{n=0}^\infty f^n sin(nğœƒ)

With [https://math.stackexchange.com/questions/2229735/show-that-sum-n-1-infty-rn-cosn-theta-dfracr-cos-theta-r21-2r-cos]

  dx = \sum_{n=0}^\infty f^n cos(nğœƒ) - 1/(1-f^2)
     = 1 + \frac{f cosğœƒ - f^2}{1 - 2f cosğœƒ + f^2} - 1/(1-f^2)
     = \frac{f cosğœƒ - f^2}{1 - 2f cosğœƒ + f^2} - f^2/(1-f^2)
  dy = \sum_{n=0}^\infty f^n sin(nğœƒ)
     = \frac{f sinğœƒ}{1 - 2f cosğœƒ + f^2}

  dx^2 + dy^2
     = ((f cosğœƒ - f^2)^2 + f^2 sin^2ğœƒ)/(1 - 2f cosğœƒ + f^2)^2
       - 2f^2/(1-f^2) (f cosğœƒ - f^2((1 - 2f cosğœƒ + f^2)
       + f^4/(1-f^2)^2
     = (f^2 - 2f^3 cosğœƒ + f^4 )/(1 - 2f cosğœƒ + f^2)^2
       - 2f^2/(1-f^2) (f cosğœƒ - f^2)/(1 - 2f cosğœƒ + f^2)
       + f^4/(1-f^2)^2
     = f^2/(1 - 2f cosğœƒ + f^2)
       - 2f^2/(1-f^2) (f cosğœƒ - f^2)/(1 - 2f cosğœƒ + f^2)
       + f^4/(1-f^2)^2
     = (f^2(1-f^2) - 2f^2(fcosğœƒ-f^2))/((1-f^2)(1 - 2f cosğœƒ + f^2))
       + f^4/(1-f^2)^2
     = f^2(1-f^2 - 2fcosğœƒ+2f^2))/((1-f^2)(1 - 2f cosğœƒ + f^2))
       + f^4/(1-f^2)^2
     = f^2/(1-f^2) + f^4/(1-f^2)^2
     = (f^2(1-f^2) + f^4)/(1-f^2)^2
     = f^2/(1-f^2)^2

which is a circle of radius f/(1-f<sup>2</sup>).
