2021-02-05 Riddler Classic
==========================
It's not clear whether solving means moving the discs to either of the
other poles or to a particular pole.  I assume it's moving to either of
the other poles since that makes the solution more tractable.

When all the discs are on the same pole, there are 2 valid moves.

When there are discs on two or three poles, there are 3 valid moves:
* move the smallest onto the largest/empty
* move the middle onto the largest/empty
* move the middle onto the smallest

For the positions with 3 valid moves, there is a 1/3 chance of moving to
each of 3 other positions, so the average number of moves to solve
from that position would be 1+1/3×(sum of the average number of moves to
solve from the 3 other positions).

So, from the start position, it is 1+1/2×(sum of the average number of moves
to solve from the 2 accessible positions (which should be equal)).

For the end positions, it is 0.

This makes a set of linear equations, or a big sparse matrix.

Tabulating the graph of the 27 positions for the 3-disc case, including
the minimum distances from the start and end positions:

For the 3-disc case, the equations are
```
m_{,,123} = 0
m_{,1,23} - m_{,,123}/3 - m_{1,,23}/3 - m_{2,1,3}/3 = 1
m_{,2,13} - m_{,12,3}/3 - m_{1,2,3}/3 - m_{2,,13}/3 = 1
m_{,12,3} - m_{,2,13}/3 - m_{1,2,3}/3 - m_{3,12,}/3 = 1
m_{,3,12} - m_{,13,2}/3 - m_{1,3,2}/3 - m_{3,,12}/3 = 1
m_{,13,2} - m_{,3,12}/3 - m_{1,3,2}/3 - m_{2,13,}/3 = 1
m_{,23,1} - m_{,123,}/3 - m_{1,23,}/3 - m_{2,3,1}/3 = 1
m_{,123,} = 0
m_{1,,23} - m_{,,123}/3 - m_{,1,23}/3 - m_{1,2,3}/3 = 1
m_{1,2,3} - m_{,12,3}/3 - m_{,2,13}/3 - m_{1,,23}/3 = 1
m_{1,3,2} - m_{,13,2}/3 - m_{,3,12}/3 - m_{1,23,}/3 = 1
m_{1,23,} - m_{,123,}/3 - m_{,23,1}/3 - m_{1,3,2}/3 = 1
m_{2,,13} - m_{,2,13}/3 - m_{12,,3}/3 - m_{2,1,3}/3 = 1
m_{2,1,3} - m_{,1,23}/3 - m_{12,,3}/3 - m_{2,,13}/3 = 1
m_{2,3,1} - m_{,23,1}/3 - m_{12,3,}/3 - m_{2,13,}/3 = 1
m_{2,13,} - m_{,13,2}/3 - m_{12,3,}/3 - m_{2,3,1}/3 = 1
m_{12,,3} - m_{12,3,}/3 - m_{2,,13}/3 - m_{2,1,3}/3 = 1
m_{12,3,} - m_{12,,3}/3 - m_{2,13,}/3 - m_{2,3,1}/3 = 1
m_{3,,12} - m_{,3,12}/3 - m_{13,,2}/3 - m_{3,1,2}/3 = 1
m_{3,1,2} - m_{13,,2}/3 - m_{23,1,}/3 - m_{3,,12}/3 = 1
m_{3,2,1} - m_{13,2,}/3 - m_{23,,1}/3 - m_{3,12,}/3 = 1
m_{3,12,} - m_{,12,3}/3 - m_{13,2,}/3 - m_{3,2,1}/3 = 1
m_{13,,2} - m_{13,2,}/3 - m_{3,,12}/3 - m_{3,1,2}/3 = 1
m_{13,2,} - m_{13,,2}/3 - m_{3,12,}/3 - m_{3,2,1}/3 = 1
m_{23,,1} - m_{123,,}/3 - m_{23,1,}/3 - m_{3,2,1}/3 = 1
m_{23,1,} - m_{123,,}/3 - m_{23,,1}/3 - m_{3,1,2}/3 = 1
m_{123,,} - m_{23,,1}/2 - m_{23,1,}/2 = 1
```
Due to symmetry when moving to either of the other poles is a solution,
m_{x,y,z} = m_{x,z,y}.
```
m_{,2,13} - m_{,3,12}/3 - m_{1,3,2}/3 - m_{2,13,}/3 = 1
m_{,3,12} - m_{,2,13}/3 - m_{1,3,2}/3 - m_{3,12,}/3 = 1
m_{,23,1} - m_{,123,}/3 - m_{1,23,}/3 - m_{2,3,1}/3 = 1
m_{,123,} = 0
m_{1,3,2} - m_{,2,13}/3 - m_{,3,12}/3 - m_{1,23,}/3 = 1
m_{1,23,} - m_{,123,}/3 - m_{,23,1}/3 - m_{1,3,2}/3 = 1
m_{2,3,1} - m_{,23,1}/3 - m_{12,3,}/3 - m_{2,13,}/3 = 1
m_{2,13,} - m_{,2,13}/3 - m_{12,3,}/3 - m_{2,3,1}/3 = 1
m_{12,3,} - m_{12,3,}/3 - m_{2,13,}/3 - m_{2,3,1}/3 = 1
m_{3,2,1} - m_{13,2,}/3 - m_{23,1,}/3 - m_{3,12,}/3 = 1
m_{3,12,} - m_{,3,12}/3 - m_{13,2,}/3 - m_{3,2,1}/3 = 1
m_{13,2,} - m_{13,2,}/3 - m_{3,12,}/3 - m_{3,2,1}/3 = 1
m_{23,1,} - m_{123,,}/3 - m_{23,1,}/3 - m_{3,2,1}/3 = 1
m_{123,,} - m_{23,1,}/2 - m_{23,1,}/2 = 1
```

I could solve this by hand, but my attempt was too error-prone, so
I'll write code to do it.  Rather than download and install some linear
algebra package, I'll just do a simple-minded upper-triangularization,
which ought to give the answer if pivots work out.  If not, I'll do
back-substitution.
