2021-10-22 Riddler Classic
==========================
Let the vertices of the equilateral triangle be at (-1,0), (1,0), and
(0,√3).  The center of the triangle is at (x₀,y₀) = (0,1/√3).

Let the vertices of the random triangle be at (x₁,y₁), (x₂,y₂), (x₃,y₃), where
```
  (x₁,y₁) = (-1+2a,0)
  (x₂,y₂) = (b-1,b√3)
  (x₃,y₃) = (1-c,c√3)
```
where a, b, and c are uniformly distributed from 0 to 1.

The random triangle contains the point (x₀,y₀) if the point is within
the angle of the vertex at (x₁,y₁) and within the angle of the vertex
at (x₂,y₂).

The point (x₀,y₀) is within the angle of the vertex at (x₁,y₁) if the
cross product of the vector from (x₁,y₁) to (x₂,y₂) with the vector from
(x₁,y₁) to (x₀,y₀) has the same sign as the cross product of the vector from
(x₁,y₁) to (x₀,y₀) with the vector from (x₁,y₁) to (x₃,y₃).  Similarly for
determining if the point is within the angle of the vertex at (x₂,y₂).

As I've formulated it, both cross products have to be negative for the center
point to be within the triangle.

The cross product of the vector from (x₁,y₁) to (x₂,y₂) with the vector
from (x₁,y₁) to (x₀,y₀) is
```
  (x₂-x₁)(y₀-y₁) - (x₀-x₁)(y₂-y₁)
    = (b-1+1-2a)(1/√3-0) - (0+1-2a)(b√3-0)
    = b/√3-2a/√3 - 3b/√3 + 6ab/√3
    = (6ab - 2b - 2a)/√3
```
or, basically, the sign of 3ab - a - b, which is negative when the center
is within the random triangle.

The cross product of the vector from (x₁,y₁) to (x₀,y₀) with the vector
from (x₁,y₁) to (x₃,y₃) is
```
  (x₀-x₁)(y₃-y₁) - (x₃-x₁)(y₀-y₁)
    = (0+1-2a)(c√3-0) - (1-c+1-2a)(1/√3-0)
    = 3c/√3-6ac/√3 - 2/√3 + 3c/√3 +6a/√3
    = (-6ac + 6a + 6c - 2)/√3
```
or, basically, the sign of -3ac + 3a + 3c - 1, which is negative when the
center is within the random triangle.

The cross product of the vector from (x₂,y₂) to (x₃,y₃) with the vector
from (x₂,y₂) to (x₀,y₀) is
```
  (x₃-x₂)(y₀-y₂) - (x₀-x₂)(y₃-y₂)
    = (1-c-b+1)(1/√3-b√3) - (0-b+1)(c√3-b√3)
    = 2/√3 - 6b/√3 - c/√3 + 3bc/√3 - b/√3 + 3b²/√3 + 3bc/√3 - 3c/√3 - 3b²/√3 + 3b/√3
    = (6bc - 4b - 4c + 2)/√3
```
or, basically, the sign of 3bc - 2b - 2c + 1, which is negative when the
center is within the random triangle.

The cross product of the vector from (x₂,y₂) to (x₀,y₀) with the vector
from (x₂,y₂) to (x₁,y₁) is
```
  (x₀-x₂)(y₁-y₂) - (x₁-x₂)(y₀-y₂)
    = (0-b+1)(0-b√3) - (-1+2a-b+1)(1/√3-b√3)
    = 3b²/√3 - 3b/√3 - 2a/√3 + 6ab/√3 + b/√3 - 3b²/√3
    = (6ab - 2a - 2b)/√3
```
or, basically, the sign of 3ab - a - b, which is negative when the center
is within the random triangle.

The probability that the center is within the random triangle is then
```
  ∫₀¹da∫₀¹db∫₀¹dc H(a + b - 3ab) H(1 + 3ac - a - c) H(2b + 2c - 1 - 3bc)
```

I'll evaluate the integrals later.
