2023-04-07 Riddler Classic
==========================
I'll assume each crew member knows their own number and does not know the
numbers of the other two.  Otherwise I can ask each if they have the highest
number.

If I ask if their number is lower than $x$, then the probability of yes is
$x$ and the probability of no is $1-x$.

The first is $g$.  If the answer is yes, the second is $s_y$, and if the
answer is no, the second is $s_n$.  Similarly, the third is $a_{yy}$,
$a_{yn}$, $a_{ny}$, or $a_{nn}$.

Enumerating the eight cases,
* With probability $gs_ya_{yy}$, I'd guess the one with the highest maximum
  number.
* With probability $gs_y(1-a_{yy})$, I'd guess Alandra.
* With probability $g(1-s_y)a_{yn}$, I'd guess Sidney.
* With probability $g(1-s_y)(1-a{yn}$, I'd guess the one with the highest
  minimum number, either Sidney or Alandra.
* With probability $(1-g)s_na_{ny}$, I'd guess Geordi.
* With probability $(1-g)s_n(1-a_{ny}$, I'd guess the one with the highest
  minimum number, either Geordi or Alandra.
* With probability $(1-g)(1-s_n)a_{nn}$, I'd guess the one with the highest
  minimum number, either Geordi or Sidney.
* With probability $(1-g)(1-s_n)(1-a_{nn}$, I'd guess the one with the
  highest minimum number.

If questions were $X$, $Y$, $Z$, where $X > Y > Z$, and the answers were all
yes, I would guess $X$, and the probability of guessing correctly would be

$$ \frac{1}{XYZ} \int_0^X dx \int_0^Y dy \int_0^Z dz H(x-y)H(x-z)
    = \frac{1}{XYZ}\left(YZ\int_Y^X dx + Z\int_Z^Y dx \int_0^x dy + \int_0^Z dx\int_0^x dy\int_0^x dz\right)
    = \frac{X-Y}X + \frac{1}{XY}\int_Z^Y dx x + \frac{1}{XYZ}\int_0^Z dx x^2
    = \frac{X-Y}X + \frac{Y^2 - Z^2}{2XY} + \frac{Z^2}{3XY}
    = 1 - \frac{Y}{X} + \frac{Y}{2X} - \frac{Z^2}{2XY} + \frac{Z^2}{3XY}
    = 1 - \frac{Y}{2X} - \frac{Z^2}{6XY} $$

If questions were $X$, $Y$, $Z$, where $X > Y > Z$, and the answers were all
no, I would guess $X$, and the probability of guessing correctly would be

$$ \frac{1}{(1-X)(1-Y)(1-Z)} \int_X^1 dx \int_Y^1 dy \int_Z^1 dz H(x-y)H(x-z)
    = \frac{1}{(1-X)(1-Y)(1-Z)} \int_X^1 dx (x - Y) (x - Z)
    = \frac{1}{(1-X)(1-Y)(1-Z)} \int_X^1 dx (x^2 - (Y + Z)x + YZ)
    = \frac{1}{(1-X)(1-Y)(1-Z)} (1/3 - X^3/3 - (Y+Z)(1/2 - X^2/2) + YZ(1-X)) $$

If the questions were $X$, $Y$, $Z$, where $X > Y > Z$, and the answer to
$X$ were no and the answer to the other two were yes, I would guess $X$,
and probability of guessing correctly would be 100%.

If the questions were $X$, $Y$, $Z$, where $X > Y > Z$, and the answer to
$Y$ were no and the answer to the other two were yes, I would guess $Y$, and
the probability of guessing correctly would be

$$ \frac{1}{X(1-Y)Z} \int_0^X dx \int_Y^1 dy \int_0^Z dz H(y-x)H(y-z)
   = \frac{1}{X(1-Y)} \int_0^X dx \int_Y^1 dy H(y-x)
   = \frac{1}{X(1-Y)}(Y(1-Y) + \int_Y^X dx \int_x^1 dy)
   = \frac{1}{X(1-Y)}(Y(1-Y) + \int_Y^X dx (1-x))
   = \frac{1}{X(1-Y)}(Y(1-Y) + Y-X - Y^2/2 + X^2/2)
   = \frac{1}{X(1-Y)}(Y-Y^2 + Y - X - Y^2/2 + X^2/2)
   = \frac{1}{X(1-Y)}(2Y-3Y^2/2 - X + X^2/2) $$

If the questions were $X$, $Y$, $Z$, where $X > Y > Z$, and the answer to
$Z$ were no and the answer to the other two were yes, I would guess $Z$, and
the probability of guessing correctly would be

$$ \frac{1}{XY(1-Z)} \int_0^X dx \int_0^Y dy \int_Z^1 dz H(z-x)H(z-y)
   = \frac{1}{XY(1-Z)}\left(Z(\int_0^Y dy \int_Z^1 dz H(z-y)) + \int_Z^z dx \int_0^Y dy \int_Z^1 dz H(z-y)\right)
   = \frac{1}{XY(1-Z)}\left(Z(\int_0^Y dy \int_Z^1 dz H(z-y)) + \int_0^Y dy \int_Z^1 dz H(z-y)(z-Z)\right)
   = \frac{1}{XY(1-Z)}\left(Z^2(1-Z)+Z(\int_Z^z dy \int_Z^1 dz) + Z\int_Z^1 dz (z-Z)+\int_Z^z dy \int_Z^1 dz (z-Z)\right)
   = \frac{1}{XY(1-Z)}\left(Z^2(1-Z)+Z(\int_Z^1 dz(z-Z)) + Z\int_Z^1 dz (z-Z)+\int_Z^1 dz (z^2-2Zz+Z^2)\right)
   = \frac{1}{XY(1-Z)}\left(Z^2(1-Z)+Z(1-Z^2-2Z(1-Z)) + \int_Z^1 dz (z^2-2Zz+Z^2)\right)
   = \frac{1}{XY(1-Z)}\left(Z^2-Z^3+Z-Z^3-2Z^2+2Z^3 + \int_Z^1 dz (z^2-2Zz+Z^2)\right)
   = \frac{1}{XY(1-Z)}\left(Z-Z^2 + 1/3-Z^3/3-Z+Z^3+Z^2-Z^3)
   = \frac{1}{XY(1-Z)}(-Z^3/3+1/3)
   = \frac{1-Z^3}{3XY(1-Z)} $$

(I did something wrong here.  This should reduce to 1 when X = Y = Z.)

If the questions were $X$, $Y$, $Z$, where $X > Y > Z$, and the answer to
$X$ were yes and the answer to the other two were no, I would guess $Y$,
and probability of guessing correctly would be

$$ \frac{1}{X(1-Y)(1-Z)} \int_0^X dx \int_Y^1 dy \int_Z^1 dz H(y-x)H(y-z)
   = \frac{1}{X(1-Y)(1-Z)} \int_Y^1 dy y (y-Z)
   = \frac{1}{X(1-Y)(1-Z)} (1/3 - Y^3/3 - Z/2 + Y^2Z/2)
   = \frac{1-Y^3}{3X(1-Y)(1-Z)} - \frac{(1+Y)Z}{2X(1-Z)} $$

(I did something wrong here.  This should reduce to 1/2 when X = Y = Z.)

If the questions were $X$, $Y$, $Z$, where $X > Y > Z$, and the answer to
$Y$ were yes and the answer to the other two were no, I would guess $X$,
and probability of guessing correctly would be

$$ \frac{1}{(1-X)Y(1-Z)} \int_X^1 dx \int_0^Y dy \int_Z^1 dz H(x-y)H(x-z)
   = \frac{1}{(1-X)(1-Z)} \int_X^1 dx (x - Z)
   = \frac{1}{(1-X)(1-Z)} (1/2 - X^2/2 - Z(1-X))
   = \frac{1+X}{2(1-Z)} - \frac{Z}{1-Z} $$

If the questions were $X$, $Y$, $Z$, where $X > Y > Z$, and the answer to
$Z$ or were yes and the answer to the other two were no, I would guess $X$,
and probability of guessing correctly would be

$$ \frac{1}{(1-X)(1-Y)Z} \int_X^1 dx \int_Y^1 dy \int_0^Z dz H(x-y)H(x-z)
   = \frac{1}{(1-X)(1-Y)} \int_X^1 dx (x - Y)
   = \frac{1}{(1-X)(1-Y)} (1/2 - X^2/2 - Y(1-X))
   = \frac{1+X}{2(1-Y)} - \frac{Y}{1-Y} $$
