2023-10-27 Fiddler
==================
If there are $N$ candidates and $n$ votes, let $P(N,n)$ be the probability
that a speaker is selected in the first round.  Then, the average number
of rounds to select a speaker is

$$ R(N,n) = P(N,n) + (1-P(N,n))(1 + R(N-1,n)) = 1 + (1-P(N,n))R(N-1,n) $$

To calculate $P$, consider the probability that an arbitrary candidate
gets $m$ votes, ${n\choose m}\frac{(N-1)^{n-m}}{N^n}$, so

$$ P(N,n) = N\sum_{m=(n+1)/2}^{n} {n\choose m}\frac{(N-1)^{n-m}}{N^n} $$

and $P(2,n) = 1$.

Using [code](20231027.hs), $R(3,221) = 617425657801704090874241098447827545759855219603833363268132854148075211286698861571172998889441418957637/308712904366595890319978599341504655567257431166409329421135089732346509723631627417356013073234099809467$, or approximately 1.9999995110943354.

Extra credit
------------
Tabulating,

|$N$|$R(N,221)$|
|---|----------|
|2  |1.0|
|3  |1.9999995110943354|
|4  |2.99999951109433|
|5  |3.99999951109433|
|6  |4.999999511094329|
|7  |5.999999511094329|
|8  |6.999999511094329|
|9  |7.999999511094329|
|10 |8.99999951109433|

Looks like there's some rounding error, since $R(10) < R(9) + 1$.

My code says $R(10) \approx R(9) + 1 - 1.4987809977035309e-49$.

Also $R(3) \approx R(2) + 1 - 4.88905664631806e-7$, and
$R(4) \approx R(3) + 1 - 5.721757074481762e-15$, so the probability
of selecting a speaker when there are more than 3 candidates is not going
to appear in the average number of rounds with 15 significant digits.

Making the rounds
-----------------
If unstable towers are allowed, then it could be infinite by, say by
alternating between larger shells and smaller shells, so I'll assume
the tower must be stable so a larger shell cannot go on top of a
smaller shell.

If there are an infinite number of shells that make a tower of height
$H(R)$, and the radius of the shell on top a shell with radius $r$ is
$fr$, then removing the bottom shell will make a tower of height
$H(fR)$, where $H(R) = H(fR) + R\sqrt{1-f^2}$.

Scaling the tower down by a factor of $f$ gives $H(fR) = fH(R)$, so

$$ H(R) = R\sqrt{\frac{1+f}{1-f}} $$

which goes to infinity as $f$ approaches 1.
