2022-12-09 Riddler Classic
==========================
The first semifinal has probability $a/(a+d)$ that A wins, and probability
$d/(a+d)$ that D wins.

The second semifinal has probability $b/(b+c)$ that B wins, and probability
$c/(b+c)$ that C wins.

The probability that A defeats B in the finals is $a^2b/((a+d)(b+c)(a+b))$.

The probability that B defeats A in the finals is $ab^2/((a+d)(b+c)(a+b))$.

The probability that A defeats C in the finals is $a^2c/((a+d)(b+c)(a+c))$.

The probability that C defeats A in the finals is $ac^2/((a+d)(b+c)(a+c))$.

The probability that D defeats B in the finals is $d^2b/((a+d)(b+c)(d+b))$.

The probability that B defeats D in the finals is $db^2/((a+d)(b+c)(d+b))$.

The probability that D defeats C in the finals is $d^2c/((a+d)(b+c)(d+c))$.

The probability that C defeats D in the finals is $dc^2/((a+d)(b+c)(d+c))$.

The average quality of the winner is

$$ \frac1C\int_0^1 da \int_0^a db \int_0^b dc \int_0^c dd \left(
      \frac{a^3b}{(a+d)(b+c)(a+b)}
    + \frac{ab^3}{(a+d)(b+c)(a+b)}
    + \frac{a^3c}{(a+d)(b+c)(a+c)}
    + \frac{ac^3}{(a+d)(b+c)(a+c)}
    + \frac{d^3b}{(a+d)(b+c)(d+b)}
    + \frac{db^3}{(a+d)(b+c)(d+b)}
    + \frac{d^3c}{(a+d)(b+c)(d+c)}
    + \frac{dc^3}{(a+d)(b+c)(d+c)}
   \right)
$$

$$ = \frac1C\int_0^1 da \int_0^a db \int_0^b dc \int_0^c dd \left(
      \frac{ab(a^2+b^2)}{(a+d)(b+c)(a+b)}
    + \frac{ac(a^2+c^2)}{(a+d)(b+c)(a+c)}
    + \frac{bd(b^2+d^2)}{(a+d)(b+c)(d+b)}
    + \frac{cd(c^2+d^2)}{(a+d)(b+c)(d+c)}
   \right)
$$

where
$$ C = \int_0^1 da \int_0^a db \int_0^b dc \int_0^c dd \left(
      \frac{ab(a+b)}{(a+d)(b+c)(a+b)}
    + \frac{ac(a+c)}{(a+d)(b+c)(a+c)}
    + \frac{bd(b+d)}{(a+d)(b+c)(d+b)}
    + \frac{cd(c+d)}{(a+d)(b+c)(d+c)}
   \right)
$$

Consider the first term,

$$ \int_0^1 da \int_0^a db \int_0^b dc \int_0^c dd\ \frac{ab(a^2+b^2)}{(a+d)(b+c)(a+b)} $$

$$ = \int_0^1 da \int_0^a db \int_0^b dc\ \frac{ab(a^2+b^2)\ln((a+c)/a)}{(b+c)(a+b)} $$

using Wolfram Alpha

$$ = \int_0^1 da \int_0^a db \frac{ab(a^2+b^2)}{a+b}\left(\Li_2(\frac{a+b}{a-b}) + \ln(\frac{a+b}a)\ln(\frac{2b}{b-a}) - \Li_2(\frac{a}{a-b})\right) $$

and that's getting too involved for me, so I'll leave it at that.
