2022-06-10 Riddler Classic
==========================
At steady-state, the probability distribution P(x) = ∫₀¹dy J(y,x)P(y)
where J(y,x) is the probability of jumping from y to x.

Let d = 20cm = 1/5.

When y is not within d of either edge, J(y,x) = H(d-|x-y|)/2d.

When 0 < y < d, J(y,x) = H(d-|x-y|)/(y+d).

When 1 > y > 1-d, J(y,x) = H(d-|x-y|)/(1-y+d).

After running some simulations, I would guess that P increases by a factor
of 2 linearly from 0 to 1/5, then is flat from 1/5 to 4/5, then decreases by
a factor of 2 linearly from 4/5 to 1.

Consider P(x) = C ((1+x/d)H(d-x) + 2H(x-d)H(1-d-x) + (1+(1-x)/d)H(x-1+d)).

Considering 2d < x < 1-2d,
* P(x) = ∫<sub>x-d</sub><sup>x+d</sup> dy 2C/2d = 2C

Considering 0 < x < d,
* P(x) = ∫<sub>0</sub><sup>d</sup> dy C(1+y/d)/(y+d) + ∫<sub>d</sub><sup>x+d</sup> dy 2C/2d
* P(x) = C + 2Cx/2d = C (1 + x/d)

Considering d < x < 2d,
* P(x) = ∫<sub>x-d</sub><sup>d</sup> dy C(1+y/d)/(y+d) + ∫<sub>d</sub><sup>x+d</sup> dy 2C/2d
* P(x) = C/d (d - (x-d)) + C/d (x+d - d) = 2C

So P(x) = C ((1+x/d)H(d-x) + 2H(x-d)H(1-d-x) + (1+(1-x)/d)H(x-1+d))
satisfies P(x) = ∫₀¹dy J(y,x)P(y).

Since ∫₀¹dx P(x) = 1, C = 1/(2-d) = 5/9.
