2022-01-21 Riddler Classic
==========================
The side length of 1 makes the radius of the circle also 1.

Let (0,0) be the center of the circle.

The upper two vertices of the large hexagon are at (±1/2,√3/2).

Let the side of the smaller hexagon be a.  Then the upper vertices of the
smaller hexagon are (±a/2,√3/2+a√3).  For them to be on the circle,
```
  a²/4 + 3/4 + 3a + 3a² = 1
  13a² + 12a - 1 = 0
```
The positive root is a = 1/13.

Extra credit
------------
Let the side of the third hexagon be b.  The upper vertices of that hexagon
are (±b/2,(1/2+1/13+b)√3) = (±b/2,(15/26+b)√3).  For them to be on the circle,
```
  b²/4 + 675/676 + 45b/13 + 3b² = 1
  169b² + 675 + 2340b + 2028b² = 676
  2197b² + 2340b - 1 = 0
```
The positive root is (-90 + √8113)/169, or about 4.27179e-4.

Let the side of the fourth hexagon be c.  The upper vertices of that hexagon
are (±c/2,(15/26+b+c)√3).  For them to be on the circle,
```
  c²/4 + 675/676 + 3b² + 3c² + 45b/13 + 45c/13 + 6bc = 1
  169c² + 675 + 2028b² + 2028c² + 2340b + 2340c + 4056bc = 676
  2197c² + (2340 + 4056b)c + 2028b² + 2340b - 1 = 0
  2197c² + (2340 + 4056b)c - 169b² = 0
  2197c² + (2340 + 12(-180 + √32452))c - (-180 + √32452)²/676 = 0
  2197c² + (180 + 12√32452)c - (64852 - 360√32452)/676 = 0
  2197c² + (180 + 12√32452)c - (16213 - 90√32452)/169 = 0
  371293c² + (30420 + 2028√32452)c - 16213 + 90√32452 = 0

  c = (-30420 - 2028√32452 + √((30420 + 2028√32452)² + 24079093636 - 133665480√32452))/742586
    = (-30420 - 2028√32452 + √(925376400 + 133468066368 + 123383520√32452 + 24079093636 - 133665480√32452))/742586
    = (-30420 - 2028√32452 + √(158472536404 - 10281960√32452))/742586
    = (-180 - 12√32452 + √(5548564 - 360√32452))/4396
    = (-90 - 6√32452 + √(1387141 - 90√32452))/2198
```
The positive root is (-90 - 12√8113 + √(1387141 - 180√8113))/2198,
or about 1.31695e-8.

In general, if the bottom of the hexagon is h above the center of the
circle, the top vertices are at (±w/2,h+w√3), and to be on the circle,
```
  w²/4 + h² + 2hw√3 + 3w² = 1
  13w² + 8hw√3 + 4h² - 4 = 0

  w = (-8h√3 + √(192h² - 208h² + 208))/26
    = (-8h√3 + √(208-16h²))/26
    = (-4h√3 + √(52-4h²))/13
```
making the top of the hexagon
```
  h + w√3 = h + (-12h + √(156-12h²))/13 = (h + √(156-12h²))/13
```
which is the bottom of the next hexagon.

Let z = 1 - h,
```
  w = (-√48 + z√48 + √(48+8z-4z²))/13
    = (-√48 + z√48 + √48√(1+z/6-z²/12))/13
    = (-√48 + z√48 + √48(1 + z/12 + ...))/13
    = z/√3 + ...
  z - w√3 = z - (-12 + 12z + √(144+24z-12z²))/13
          = (12 - z - √(144+24z-12z²))/13
	  = (12 - z - 12√(1 + z/6 - z²/12))/13
	  = (12 - z - 12(1 + z/12 - z²/24 - z²/288 + ...))/13
	  = z²/24 + ...
```

With this approximation, the next few hexagons would have sides that
are approximately 1.25e-17, 1.13e-35, 9.23e-72, 6.15e-144, 2.73e-288.
